test/sort.lean
@@ -1,12 +1,32 @@
 import tactic.sort
-import data.polynomial.basic
+import data.polynomial.degree
 
 open polynomial tactic interactive
 open_locale polynomial
 
-variables {R : Type*} [semiring R] (f g h : R[X]) {r s t u : R} (r0 : t ≠ 0)
+variables {R : Type*} [semiring R] (f g h : R[X]) {r s t u : R}
 
-lemma pro
+example (s0 : s ≠ 0) (m n : ℕ) (mn : m < n) (m1 : 1 ≤ m) :
+  (C r * X ^ m + (5 + C s * X ^ n) + m * X + 37 * X).nat_degree = n :=
+begin
+  -- move `C s * X ^ n` to the right, since it is the term with highest degree
+  -- we also move `m * X` and `37 * X` to the left, to collect them in a single summand
+  sort_summands [C s * X ^ n, ← ↑m * (X : R[X]), ← 37 * (X : R[X])],
+  rw [← add_mul, nat_degree_add_eq_right_of_nat_degree_lt, nat_degree_C_mul_X_pow _ _ s0],
+  rw [nat_degree_C_mul_X_pow _ _ s0],
+  -- what is left has degree at most `m < n`, so let's inform Lean
+  refine lt_of_le_of_lt _ mn,
+  -- all summands are now of degree at most `m`, so we break the sum into pieces
+  repeat { refine (nat_degree_add_le _ _).trans _,
+    refine max_le _ _ };
+    try { simp only [nat_degree_one, zero_le], done },
+  -- we have now focused on the two "interesting" terms
+  { convert (nat_degree_C_mul_X_pow_le (m + 37 : R) _).trans m1;
+    simp only [map_add, C_eq_nat_cast, C_bit1, C_bit0, map_one, pow_one] },
+  { exact nat_degree_C_mul_X_pow_le _ _ }
+end
+
+example
   (hp : (monomial 1) u + (g + (monomial 5) 1) + 5 * X + ((monomial 0) s + (monomial 2) t + f) +
   (monomial 8) 1 = (3 * X + (monomial 8) 1 + (monomial 6) (t + 1)) + f + h + ((monomial 0) s +
   (monomial 1) u) + (monomial 5) 1) :
@@ -20,6 +40,16 @@ begin
   sort_summands [(5 * X : R[X]), monomial 2 t, monomial 0 s],
   sort_summands at ⊢ hp,
   assumption,
+end
+
+example (hp : f = g) :
+  7 + f + (C r * X ^ 3 + 42) + X ^ 5 * h = C r * X ^ 3 + h * X ^ 5 + g + 7 + 42 :=
+begin
+  -- we move `f, g` to the right of their respective sides, so `congr` helps us remove the
+  -- repeated term
+  sort_summands [f, g],
+  congr' 2, -- takes care of using assumption `hp`
+  exact X_pow_mul,
 end
 
 example (hp : f = g) :
